compiler/src/Translation/ImpJsontoJavaScriptAst.v
@@ -22,154 +22,188 @@ Require Import Utils.
 Require Import Imp.
 Require Import ImpJson.
 Require Import JavaScriptAstRuntime.
+Require Import ForeignEJSONtoJavaScriptAst.
 
 Section ImpJsontoJavaScriptAst.
   Import ListNotations.
 
+  Section Util.
+    Definition scope l := stat_block l. (* XXX TODO XXX *)
+    Definition prog_to_string (x: prog) : string := "". (* XXX TODO: prog_to_string XXX *)
+
+    Definition mk_expr_error := expr_literal literal_null.
+    Definition mk_unary_expr (f:expr -> expr) (el:list expr) : expr :=
+      match el with
+      | [e] => f e
+      | _ => mk_expr_error
+      end.
+
+    Definition mk_unary_op (op:unary_op) (el:list expr) : expr :=
+      mk_unary_expr (expr_unary_op op) el.
+    
+    Definition mk_binary_expr (f:expr -> expr -> expr) (el:list expr) : expr :=
+      match el with
+      | [e1;e2] => f e1 e2
+      | _ => mk_expr_error
+      end.
+
+    Definition mk_binary_op (op:binary_op) (el:list expr) : expr :=
+      mk_binary_expr (fun e1 e2 => expr_binary_op e1 op e2) el.
+
+    Definition mk_object (atts:list string) (el:list expr) : expr :=
+      match zip atts el with
+      | Some l =>
+        expr_object
+          (List.map
+             (fun (entry: string * expr) =>
+                let (lbl, e) := entry in
+                (propname_identifier lbl, propbody_val e))
+             l)
+      | None => mk_expr_error
+      end.
+
+    Definition mk_runtime_call (op: imp_json_runtime_op) (el: list expr) :=
+      call_runtime (string_of_json_runtime_op op) el.
+
+    Definition imp_json_op_to_js_ast (op:imp_json_op) el : expr :=
+      match op with
+      | EJSONOpNot => mk_unary_op unary_op_not el
+      | EJSONOpNeg => mk_unary_op unary_op_neg el
+      | EJSONOpAnd => mk_binary_op binary_op_and el
+      | EJSONOpOr => mk_binary_op binary_op_or el
+      | EJSONOpLt => mk_binary_op binary_op_lt el
+      | EJSONOpLe => mk_binary_op binary_op_le el
+      | EJSONOpGt => mk_binary_op binary_op_gt el
+      | EJSONOpGe => mk_binary_op binary_op_ge el
+      | EJSONOpAddString => mk_binary_op binary_op_add el
+      | EJSONOpAddNumber => mk_binary_op binary_op_add el
+      | EJSONOpSub => mk_binary_op binary_op_sub el
+      | EJSONOpDiv => mk_binary_op binary_op_div el
+      | EJSONOpMult => mk_binary_op binary_op_mult el
+      | EJSONOpStrictEqual => mk_binary_op binary_op_strict_equal el
+      | EJSONOpStrictDisequal => mk_binary_op binary_op_strict_disequal el
+      | EJSONOpArray => expr_array (List.map Some el)
+      | EJSONOpArrayLength => mk_unary_expr (fun e => expr_member e  "length") el
+      | EJSONOpArrayPush => mk_binary_expr array_push el
+      | EJSONOpArrayAccess => mk_binary_expr array_get el
+      | EJSONOpObject atts => mk_object atts el
+      | EJSONOpAccess att => mk_binary_expr expr_access (el++[expr_literal (literal_string att)])
+      | EJSONOpHasOwnProperty att => mk_binary_expr object_hasOwnProperty (el++[expr_literal (literal_string att)])
+      | EJSONOpToString => expr_call (expr_identifier "toString") el
+      | EJSONOpMathMin => expr_call (expr_member (expr_identifier "Math") "min") el
+      | EJSONOpMathMax => expr_call (expr_member (expr_identifier "Math") "max") el
+      | EJSONOpMathMinApply =>
+        expr_call
+          (expr_member (expr_member (expr_identifier "Math") "min") "apply")
+          (expr_identifier "Math" :: el)
+      | EJSONOpMathMaxApply =>
+        expr_call
+          (expr_member (expr_member (expr_identifier "Math") "max") "apply")
+          (expr_identifier "Math" :: el)
+      | EJSONOpMathPow => expr_call (expr_member (expr_identifier "Math") "pow") el
+      | EJSONOpMathExp => expr_call (expr_member (expr_identifier "Math") "exp") el
+      | EJSONOpMathAbs => expr_call (expr_member (expr_identifier "Math") "abs") el
+      | EJSONOpMathLog => expr_call (expr_member (expr_identifier "Math") "log2") el
+      | EJSONOpMathLog10 => expr_call (expr_member (expr_identifier "Math") "log10") el
+      | EJSONOpMathSqrt => expr_call (expr_member (expr_identifier "Math") "sqrt") el
+      | EJSONOpMathCeil => expr_call (expr_member (expr_identifier "Math") "ceil") el
+      | EJSONOpMathFloor => expr_call (expr_member (expr_identifier "Math") "floor") el
+      | EJSONOpMathTrunc => expr_call (expr_member (expr_identifier "Math") "trunc") el
+      end.
+
+  End Util.
+
   (** Translation *)
+  Section Translation.
 
-  Definition scope l := stat_block l. (* XXX TODO XXX *)
-  Definition prog_to_string (x: prog) : string := "". (* XXX TODO: prog_to_string XXX *)
+    Context {ft:foreign_ejson}.
+    Context {ftjast:foreign_ejson_to_ajavascript}.
+  
+    Fixpoint ejson_to_js_ast (json: ejson) : expr :=
+      match json with
+      | ejnull => expr_literal literal_null
+      | ejnumber n => expr_literal (literal_number n)
+      | ejbigint n => expr_literal (literal_number (float_of_int n)) (* XXX Could be replaced by JavaScript BigInt some fix to JsAst XXX *)
+      | ejbool b => expr_literal (literal_bool b)
+      | ejstring s => expr_literal (literal_string s)
+      | ejarray a =>
+        let a :=
+            List.map
+              (fun v => Some (ejson_to_js_ast v))
+              a
+        in
+        expr_array a
+      | ejobject o =>
+        expr_object
+          (List.map
+             (fun (prop: (string * EJSON.ejson)) =>
+                let (x, v) := prop in
+                (propname_identifier x, propbody_val (ejson_to_js_ast v)))
+             o)
+      | ejforeign fd =>
+        foreign_ejson_to_ajavascript_expr fd
+      end.
 
-  Definition mk_expr_error := expr_literal literal_null.
-  Definition mk_unary_expr (f:expr -> expr) (el:list expr) : expr :=
-    match el with
-    | [e] => f e
-    | _ => mk_expr_error
-    end.
+    Fixpoint imp_json_expr_to_js_ast (exp: imp_json_expr) : expr :=
+      match exp with
+      | ImpExprError v => mk_expr_error
+      | ImpExprVar v => expr_identifier v
+      | ImpExprConst j => ejson_to_js_ast j
+      | ImpExprOp op el => imp_json_op_to_js_ast op (map imp_json_expr_to_js_ast el)
+      | ImpExprRuntimeCall rop el => mk_runtime_call rop (map imp_json_expr_to_js_ast el)
+      end.
 
-  Definition mk_unary_op (op:unary_op) (el:list expr) : expr :=
-    mk_unary_expr (expr_unary_op op) el.
+    Definition decl_to_js_ast (d : var * option imp_expr) :=
+      match d with
+      | (x, None) => (x, None)
+      | (x, Some e) => (x, Some (imp_json_expr_to_js_ast e))
+      end.
 
-  Definition mk_binary_expr (f:expr -> expr -> expr) (el:list expr) : expr :=
-    match el with
-    | [e1;e2] => f e1 e2
-    | _ => mk_expr_error
-    end.
+    Fixpoint imp_json_stmt_to_js_ast (stmt: imp_json_stmt): stat :=
+      match stmt with
+      | ImpStmtBlock decls stmts =>
+        scope
+          (stat_let_decl (List.map decl_to_js_ast decls) :: (List.map imp_json_stmt_to_js_ast stmts))
+      | ImpStmtAssign x e =>
+        stat_expr (expr_assign (expr_identifier x) None (imp_json_expr_to_js_ast e))
+      | ImpStmtFor x e s =>
+        stat_for_in_let nil x None (imp_json_expr_to_js_ast e)
+                        (imp_json_stmt_to_js_ast s)
+      | ImpStmtForRange x e1 e2 s =>
+        stat_for_let
+          nil
+          [ (x, Some (imp_json_expr_to_js_ast e1)) ]
+          (Some (expr_binary_op (expr_identifier x) binary_op_lt (imp_json_expr_to_js_ast e2)))
+          (Some (expr_unary_op unary_op_post_incr (expr_identifier x)))
+          (imp_json_stmt_to_js_ast s)
+      | ImpStmtIf e s1 s2 =>
+        stat_if
+          (imp_json_expr_to_js_ast e)
+          (imp_json_stmt_to_js_ast s1)
+          (Some (imp_json_stmt_to_js_ast s2))
+      end.
 
-  Definition mk_binary_op (op:binary_op) (el:list expr) : expr :=
-    mk_binary_expr (fun e1 e2 => expr_binary_op e1 op e2) el.
+    Definition imp_json_function_to_js_ast (f: imp_function) : list string * funcbody :=
+      match f with
+      | ImpFun v s ret =>
+        let body := imp_json_stmt_to_js_ast s in
+        let ret := scope (body :: stat_return (Some (expr_identifier ret)) :: nil) in
+        let prog :=
+            prog_intro strictness_true [ element_stat ret ]
+        in
+        ([v], funcbody_intro prog (prog_to_string prog))
+      end.
 
-  Definition mk_object (atts:list string) (el:list expr) : expr :=
-    match zip atts el with
-    | Some l =>
-      expr_object
-        (List.map
-           (fun (entry: string * expr) =>
-              let (lbl, e) := entry in
-              (propname_identifier lbl, propbody_val e))
-           l)
-    | None => mk_expr_error
-    end.
-
-  Definition mk_runtime_call (op: imp_json_runtime_op) (el: list expr) :=
-    call_runtime (string_of_json_runtime_op op) el.
-
-  Definition imp_json_op_to_js_ast (op:imp_json_op) el : expr :=
-    match op with
-    | JSONOpNot => mk_unary_op unary_op_not el
-    | JSONOpNeg => mk_unary_op unary_op_neg el
-    | JSONOpAnd => mk_binary_op binary_op_and el
-    | JSONOpOr => mk_binary_op binary_op_or el
-    | JSONOpLt => mk_binary_op binary_op_lt el
-    | JSONOpLe => mk_binary_op binary_op_le el
-    | JSONOpGt => mk_binary_op binary_op_gt el
-    | JSONOpGe => mk_binary_op binary_op_ge el
-    | JSONOpAddString => mk_binary_op binary_op_add el
-    | JSONOpAddNumber => mk_binary_op binary_op_add el
-    | JSONOpSub => mk_binary_op binary_op_sub el
-    | JSONOpDiv => mk_binary_op binary_op_div el
-    | JSONOpMult => mk_binary_op binary_op_mult el
-    | JSONOpStrictEqual => mk_binary_op binary_op_strict_equal el
-    | JSONOpStrictDisequal => mk_binary_op binary_op_strict_disequal el
-    | JSONOpArray => expr_array (List.map Some el)
-    | JSONOpArrayLength => mk_unary_expr (fun e => expr_member e  "length") el
-    | JSONOpArrayPush => mk_binary_expr array_push el
-    | JSONOpArrayAccess => mk_binary_expr array_get el
-    | JSONOpObject atts => mk_object atts el
-    | JSONOpAccess att => mk_binary_expr expr_access (el++[expr_literal (literal_string att)])
-    | JSONOpHasOwnProperty att => mk_binary_expr object_hasOwnProperty (el++[expr_literal (literal_string att)])
-    | JSONOpToString => expr_call (expr_identifier "toString") el
-    | JSONOpMathMin => expr_call (expr_member (expr_identifier "Math") "min") el
-    | JSONOpMathMax => expr_call (expr_member (expr_identifier "Math") "max") el
-    | JSONOpMathMinApply =>
-      expr_call
-        (expr_member (expr_member (expr_identifier "Math") "min") "apply")
-        (expr_identifier "Math" :: el)
-    | JSONOpMathMaxApply =>
-      expr_call
-        (expr_member (expr_member (expr_identifier "Math") "max") "apply")
-        (expr_identifier "Math" :: el)
-    | JSONOpMathPow => expr_call (expr_member (expr_identifier "Math") "pow") el
-    | JSONOpMathExp => expr_call (expr_member (expr_identifier "Math") "exp") el
-    | JSONOpMathAbs => expr_call (expr_member (expr_identifier "Math") "abs") el
-    | JSONOpMathLog => expr_call (expr_member (expr_identifier "Math") "log2") el
-    | JSONOpMathLog10 => expr_call (expr_member (expr_identifier "Math") "log10") el
-    | JSONOpMathSqrt => expr_call (expr_member (expr_identifier "Math") "sqrt") el
-    | JSONOpMathCeil => expr_call (expr_member (expr_identifier "Math") "ceil") el
-    | JSONOpMathFloor => expr_call (expr_member (expr_identifier "Math") "floor") el
-    | JSONOpMathTrunc => expr_call (expr_member (expr_identifier "Math") "trunc") el
-    end.
-
-  Fixpoint imp_json_expr_to_js_ast (exp: imp_json_expr) : expr :=
-    match exp with
-    | ImpExprError v => mk_expr_error
-    | ImpExprVar v => expr_identifier v
-    | ImpExprConst j => json_to_js_ast j
-    | ImpExprOp op el => imp_json_op_to_js_ast op (map imp_json_expr_to_js_ast el)
-    | ImpExprRuntimeCall rop el => mk_runtime_call rop (map imp_json_expr_to_js_ast el)
-    end.
-
-  Definition decl_to_js_ast (d : var * option imp_expr) :=
-    match d with
-    | (x, None) => (x, None)
-    | (x, Some e) => (x, Some (imp_json_expr_to_js_ast e))
-    end.
-
-  Fixpoint imp_json_stmt_to_js_ast (stmt: imp_json_stmt): stat :=
-    match stmt with
-    | ImpStmtBlock decls stmts =>
-      scope
-        (stat_let_decl (List.map decl_to_js_ast decls) :: (List.map imp_json_stmt_to_js_ast stmts))
-    | ImpStmtAssign x e =>
-      stat_expr (expr_assign (expr_identifier x) None (imp_json_expr_to_js_ast e))
-    | ImpStmtFor x e s =>
-      stat_for_in_let nil x None (imp_json_expr_to_js_ast e)
-                      (imp_json_stmt_to_js_ast s)
-    | ImpStmtForRange x e1 e2 s =>
-      stat_for_let
-        nil
-        [ (x, Some (imp_json_expr_to_js_ast e1)) ]
-        (Some (expr_binary_op (expr_identifier x) binary_op_lt (imp_json_expr_to_js_ast e2)))
-        (Some (expr_unary_op unary_op_post_incr (expr_identifier x)))
-        (imp_json_stmt_to_js_ast s)
-    | ImpStmtIf e s1 s2 =>
-      stat_if
-        (imp_json_expr_to_js_ast e)
-        (imp_json_stmt_to_js_ast s1)
-        (Some (imp_json_stmt_to_js_ast s2))
-    end.
-
-  Definition imp_json_function_to_js_ast (f: imp_function) : list string * funcbody :=
-    match f with
-    | ImpFun v s ret =>
-      let body := imp_json_stmt_to_js_ast s in
-      let ret := scope (body :: stat_return (Some (expr_identifier ret)) :: nil) in
-      let prog :=
-          prog_intro strictness_true [ element_stat ret ]
-      in
-      ([v], funcbody_intro prog (prog_to_string prog))
-    end.
-
-  Definition imp_json_to_js_ast (q: imp) : list funcdecl :=
-    match q with
-    | ImpLib l =>
-      List.map
-        (fun (decl: string * imp_function) =>
-           let (x, f) := decl in
-           let (args, body) := imp_json_function_to_js_ast f in
-           funcdecl_intro x args body)
-        l
-    end.
+    Definition imp_json_to_js_ast (q: imp) : list funcdecl :=
+      match q with
+      | ImpLib l =>
+        List.map
+          (fun (decl: string * imp_function) =>
+             let (x, f) := decl in
+             let (args, body) := imp_json_function_to_js_ast f in
+             funcdecl_intro x args body)
+          l
+      end.
+  End Translation.
 
 End ImpJsontoJavaScriptAst.
